.

LCNova.v
@@ -1717,7 +1717,7 @@ Module UntypedLambdaCalculus.
     forall M1 : Term,
     forall M2 : Term,
     forall dbctx : list (IVar * IVar),
-    (forall z1 : IVar, forall z2 : IVar, IsSubtermOf (Var z1) M1 -> IsSubtermOf (Var z2) M2 -> forall dbctx' : list (IVar * IVar), ScopeTrans (map fst dbctx') (Var z1) M1 (map fst dbctx) -> ScopeTrans (map snd dbctx') (Var z2) M2 (map snd dbctx) -> WellFormedDBCtx dbctx' (Var z1) (Var z2) ) ->
+    (forall z1 : IVar, forall z2 : IVar, IsSubtermOf (Var z1) M1 -> IsSubtermOf (Var z2) M2 -> forall dbctx' : list (IVar * IVar), ScopeTrans (map fst dbctx') (Var z1) M1 (map fst dbctx) -> ScopeTrans (map snd dbctx') (Var z2) M2 (map snd dbctx) -> WellFormedDBCtx dbctx' (Var z1) (Var z2)) ->
     WellFormedDBCtx dbctx M1 M2.
   Proof.
     intros M1.
@@ -1782,6 +1782,41 @@ Module UntypedLambdaCalculus.
         apply H2.
         apply ScopeTransLam0.
         apply H3.
+  Qed.
+
+  Fixpoint makeScopeTrans (Gamma : list IVar) (M : Term) (N : Term) (X : IsSubtermOf M N) : list IVar :=
+    match X with
+    | IsSubtermOfRefl M0 => Gamma
+    | IsSubtermOfApp1 M0 P1 P2 X1 => makeScopeTrans Gamma M0 P1 X1
+    | IsSubtermOfApp2 M0 P1 P2 X2 => makeScopeTrans Gamma M0 P2 X2
+    | IsSubtermOfLam0 M0 y Q X0 => makeScopeTrans (y :: Gamma) M0 Q X0
+    end
+  .
+
+  Lemma makeScopeTrans_property1 :
+    forall M : Term,
+    forall N : Term,
+    forall X : IsSubtermOf M N,
+    forall Gamma : list IVar,
+    ScopeTrans (makeScopeTrans Gamma M N X) M N Gamma.
+  Proof.
+    intros M N X.
+    induction X.
+    - simpl.
+      intros.
+      apply ScopeTransRefl.
+    - simpl.
+      intros.
+      apply ScopeTransApp1.
+      apply IHX.
+    - simpl.
+      intros.
+      apply ScopeTransApp2.
+      apply IHX.
+    - simpl.
+      intros.
+      apply ScopeTransLam0.
+      apply IHX.
   Qed.
 
   End AlphaEquiv.
